Practico 7 - ejercicio 6 terminado.

practico7/Actions.v
@@ -3,3 +3,158 @@
  * (Como transformadores de estado)
  ******************************************************************)
 
+Require Import State.
+
+Section Actions.
+
+Inductive Action : Set
+:=   read : vadd -> Action
+   | write : vadd -> value -> Action
+   | chmod : Action.
+
+
+Definition pre_read (s: state) (va: vadd): Prop
+:= (ctxt_vadd_accessible ctxt va = true)
+/\ aos_activity s = running
+/\ (exists (ma: madd), va_mapped_to_ma s va ma 
+    /\ is_RW (page_content ((memory s) ma))).
+
+Definition post_read (s s':state): Prop
+:= s = s'.
+
+Definition pre_write (s: state) (va: vadd) (val: value)
+:= (ctxt_vadd_accessible ctxt va = true)
+/\ aos_activity s = running
+/\ (exists (ma: madd), va_mapped_to_ma s va ma
+                       /\ is_RW (page_content ((memory s) ma))).
+
+Definition post_write (s s': state) (va: vadd) (val: value) : Prop
+:= (exists (ma:madd), va_mapped_to_ma s va ma
+/\ (memory s') = (update (memory s) ma (Page (RW val) (Os (active_os s))))
+/\ active_os s = active_os s'
+/\ aos_exec_mode s = aos_exec_mode s'
+/\ aos_activity s = aos_activity s'
+/\ oss s = oss s'
+/\ hypervisor s = hypervisor s'
+/\ forall (i:madd), (ma <> i) /\ ((memory s) i = (memory s') i)).
+
+Definition pre_chmod (s: state): Prop
+:= aos_activity s = waiting 
+/\ hcall ((oss s) (active_os s)) = None.
+
+Definition post_chmod (s s': state): Prop
+:= ((ctxt_oss ctxt (active_os s) = true)
+/\ active_os s' = active_os s
+/\ aos_exec_mode s' = svc /\ aos_exec_mode s = usr
+/\ aos_activity s' = running /\ aos_activity s = waiting
+/\ oss s' = oss s
+/\ hypervisor s' = hypervisor s
+/\ memory s' = memory s)
+\/ (ctxt_oss ctxt (active_os s) = false
+   /\ active_os s' = active_os s
+   /\ aos_exec_mode s' = usr /\ aos_exec_mode s = svc
+   /\ aos_activity s' = running /\ aos_activity s = waiting
+   /\ oss s' = oss s
+   /\ hypervisor s' = hypervisor s
+   /\ memory s' = memory s). 
+
+
+Definition Pre (s:state) (a: Action) : Prop
+:=  match a with
+       read va      => pre_read s va
+     | write va val => pre_write s va val
+     | chmod        => pre_chmod s  
+    end.
+
+Definition Post (s: state) (a: Action) (s': state): Prop
+:=  match a with
+       read _       => post_read s s'
+     | write va val => post_write s s' va val
+     | chmod        => post_chmod s s'
+    end.
+
+
+Definition valid_state_prop_3 (s: state) : Prop
+:= (ctxt_oss ctxt (active_os s) = true
+/\ (aos_activity s) = running)
+   \/ (aos_activity s = waiting) -> aos_exec_mode s = svc.
+
+Definition valid_state_prop_5 (s:state) : Prop
+:= (forall (o: os_ident) (pa: padd), page_owned_by ((memory s) ((hypervisor s) o pa)) = Os o)
+/\ forall (o: os_ident) (pa pa': padd), (hypervisor s) o pa = (hypervisor s) o pa' -> pa = pa'.
+
+Definition valid_state_prop_6 (s: state) : Prop
+:= forall (o: os_ident) (pag: page) (va_to_ma: vadd -> madd), page_owned_by pag = Os o 
+/\ page_content pag = PT va_to_ma ->
+forall (va: vadd), (ctxt_vadd_accessible ctxt va = true -> 
+                                       page_owned_by ((memory s) (va_to_ma va)) = Os o)
+                                       /\ (ctxt_vadd_accessible ctxt va = false ->
+                                           page_owned_by ((memory s) (va_to_ma va)) = Hyp).
+
+Definition valid_state (s: state) : Prop
+:= valid_state_prop_3 s /\ valid_state_prop_5 s /\ valid_state_prop_6 s.
+
+Inductive one_step_execution : state -> Action -> state -> Prop
+:= one_step_execution0 : forall (s s': state) (a: Action),
+                         valid_state s -> Pre s a -> Post s a s' -> one_step_execution s a s'.
+
+
+Theorem e76 (s s': state) (a: Action) : one_step_execution s a s' -> valid_state_prop_3 s'.
+Proof.
+  intros.
+  inversion H.
+  inversion H0.
+  unfold valid_state_prop_3; intros.
+  destruct a.
+    (* read *)
+    inversion H2.
+    rewrite -> H9 in H6.
+    apply H6; assumption.
+
+    (* write *)
+    elim H6; intros;
+
+    inversion H2;
+    elim H9; intros;
+    elim H11; intros;
+    elim H13; intros;
+    elim H15; intros.
+
+    symmetry; assumption.
+
+    elim H17; intros.
+    rewrite -> H14, H18; assumption.
+
+    (* chmod *)
+    inversion H2.
+    
+    elim H9; intros;
+    elim H11; intros;
+    elim H13; intros; assumption.
+
+    elim H8; intros.
+
+    elim H9; intros;
+    elim H12; intros;
+    elim H10; intros.
+    rewrite <- H13 in H11.
+    rewrite -> H15 in H11; discriminate.
+
+    elim H9; intros;
+    elim H12; intros;
+    elim H14; intros;
+    elim H16; intros;
+    elim H18; intros.
+    rewrite -> H19 in H10; discriminate.
+Qed.
+
+Lemma Read_isolation (s s': state) (va: vadd) :
+one_step_execution s (read va) s' -> 
+exists (ma: madd), va_mapped_to_ma s va ma
+                   /\ exists (pg: page), pg = (memory s) ma /\ (page_owned_by pg) = Os (active_os s).
+Proof.
+
+
+Qed. 
+
+End Actions.
