practico7/State.v
@@ -41,9 +41,70 @@ Record context : Set :=
   Context
     {(** una direcci\u00f3n virtual es accesible, i.e. no est\u00e1 reserveda 
          por el Hypervisor *)
-       ctxt_vadd_accessible: vadd -> bool;
+       ctxt_vadd_accessible: vadd -> bool; 
      (** guest Oss (Confiable/No Confiable) **)
        ctxt_oss : os_ident -> bool
     }.
+
+
+Inductive exec_mode : Set := usr | svc.
+
+Inductive os_activity : Set := running | waiting.
+
+Record os : Set :=
+  Os_
+    {  curr_page : padd;
+       hcall : option Hyperv_call
+    }.
+
+Definition oss_map : Set := os_ident -> os.
+
+Definition hypervisor_map : Set := os_ident -> (padd -> madd).
+
+Inductive content : Set
+:=     PT (va_to_ma : vadd -> madd)
+     | RW (v : value)
+     | Other.
+
+Definition is_RW (c:content) : Prop 
+:=  match c with
+       RW _ => True
+     | _ => False
+    end.
+
+Inductive page_owner : Set
+:=   Hyp
+   | Os (osi : os_ident)
+   | No_Owner.
+
+Record page : Set :=
+  Page
+    {  page_content : content;
+       page_owned_by : page_owner
+    }.
+
+Definition system_memory : Set := madd -> page.
+
+(* Estado de la m\u00e1quina *)
+Record state : Set :=
+  State
+    { active_os : os_ident;
+      aos_exec_mode : exec_mode;
+      aos_activity : os_activity;
+      oss : oss_map;
+      hypervisor : hypervisor_map;
+      memory : system_memory
+    }.
+
+Parameter ctxt : context.
+
+Definition va_mapped_to_ma (s: state) (va: vadd) (ma: madd) : Prop
+:= exists (p: page) (vtm: vadd -> madd), page_content p = PT vtm /\
+   vtm va = ma.
+
+Definition update (m:system_memory) (ma:madd) (p: page) : system_memory
+:= fun (ma': madd) => if (madd_eq ma ma')
+                      then p
+                      else m ma.
 
 End State.
